problem 4

HumanEvalLean/HumanEval4.lean
@@ -1,5 +1,115 @@
-def mean_absolute_deviation : Unit :=
-  ()
+module
+
+import Std
+open Std
+
+/-! ## Missing API -/
+
+theorem List.sum_eq_foldl [Zero α] [Add α]
+    [Associative (α := α) (· + ·)][Commutative (α := α) (· + ·)]
+    [LawfulLeftIdentity (· + ·) (0 : α)]
+    {xs : List α} :
+    xs.sum = xs.foldl (init := 0) (· + ·) := by
+  conv => lhs; rw [← List.reverse_reverse (as := xs)]
+  rw [List.sum_reverse, List.sum_eq_foldr, List.foldr_reverse]
+  simp only [Commutative.comm]
+
+def Std.Iter.sum [Add β] [Zero β] [Iterator α Id β] [IteratorLoop α Id Id]
+    (it : Iter (α := α) β) : β :=
+  it.fold (init := 0) (· + ·)
+
+theorem Std.Iter.sum_toList [Add β] [Zero β]
+    [Associative (α := β) (· + ·)] [Commutative (α := β) (· + ·)]
+    [LawfulLeftIdentity (· + ·) (0 : β)]
+    [Iterator α Id β] [IteratorLoop α Id Id]
+    [LawfulIteratorLoop α Id Id] [Iterators.Finite α Id] {it : Iter (α := α) β} :
+    it.toList.sum = it.sum := by
+  simp only [Iter.sum, ← Iter.foldl_toList, List.sum_eq_foldl]
+
+theorem Array.size_singleton {x : α} :
+    #[x].size = 1 := by
+  simp
+
+@[simp, grind =]
+theorem Array.sum_singleton [Add α] [Zero α] [LawfulRightIdentity (· + ·) (0 : α)] {x : α} :
+    #[x].sum = x := by
+  simp [Array.sum_eq_foldr, LawfulRightIdentity.right_id x]
+
+-- Library defect: remove the `LeftIdentity` parameter from Array.sum_append
+
+@[simp, grind =]
+theorem Array.sum_push [Add α] [Zero α]
+    [Associative (α := α) (· + ·)]
+    [LawfulIdentity (· + ·) (0 : α)]
+    {xs : Array α} {x : α} :
+    (xs.push x).sum = xs.sum + x := by
+  simp [Array.sum_eq_foldr, LawfulRightIdentity.right_id, LawfulLeftIdentity.left_id,
+    ← Array.foldr_assoc]
+
+def Rat.abs (x : Rat) :=
+  if 0 ≤ x then x else - x
+
+instance Rat.instAssociativeHAdd : Associative (α := Rat) (· + ·) := ⟨Rat.add_assoc⟩
+instance Rat.instCommutativeHAdd : Commutative (α := Rat) (· + ·) := ⟨Rat.add_comm⟩
+instance : Std.LawfulIdentity (· + ·) (0 : Rat) where
+  left_id := Rat.zero_add
+  right_id := Rat.add_zero
+
+/-! ## Implementation -/
+
+def mean (xs : Array Rat) : Rat :=
+  xs.sum / xs.size
+
+def meanAbsoluteDeviation (xs : Array Rat) : Rat :=
+  let mean := mean xs
+  (xs.iter
+    |>.map (fun x => (x - mean).abs)
+    |>.sum) / xs.size
+
+/-! ## Tests -/
+
+example : meanAbsoluteDeviation #[(1 : Rat), 2, 3] = (2 : Rat) / 3 := by native_decide
+example : meanAbsoluteDeviation #[(1 : Rat), 2, 3, 4] = 1 := by native_decide
+example : meanAbsoluteDeviation #[(1 : Rat), 2, 3, 4, 5] = (6 : Rat) / 5 := by native_decide
+
+/-!
+## Verification
+
+In order to verify the implementation, we point to library lemmas verifying `Array.sum`,
+`Array.size` and `Array.map`. Then we show that `mean` is actually the quotient of `sum` and `size`
+and that `meanAbsoluteDeviation` computes the mean of absolute deviations from the mean,
+expressed using said three library functions.
+-/
+
+section API
+
+variable {x : Rat} {xs ys : Array Rat} {f : Rat → β}
+
+example : (#[] : Array Rat).sum = 0 := Array.sum_empty
+example : (#[x]).sum = x := Array.sum_singleton
+example : (xs.push x).sum = xs.sum + x := Array.sum_push
+example : (xs ++ ys).sum = xs.sum + ys.sum := Array.sum_append
+
+example : (#[] : Array Rat).size = 0 := Array.size_empty
+example : (#[x]).size = 1 := Array.size_singleton
+example : (xs.push x).size = xs.size + 1 := Array.size_push _
+example : (xs ++ ys).size = xs.size + ys.size := Array.size_append
+
+example : (#[] : Array Rat).map f = #[] := Array.map_empty
+example : #[x].map f = #[f x] := Array.map_singleton
+example : (xs.push x).map f = (xs.map f).push (f x) := Array.map_push
+example : (xs ++ ys).map f = xs.map f ++ ys.map f := Array.map_append
+
+end API
+
+theorem mean_spec {xs : Array Rat} :
+    mean xs = xs.sum / xs.size := by
+  simp [mean]
+
+theorem meanAbsoluteDeviation_spec {xs : Array Rat} :
+    meanAbsoluteDeviation xs =
+      mean (xs.map (fun x => (x - mean xs).abs)) := by
+  simp [meanAbsoluteDeviation, mean, ← Iter.sum_toList, ← Array.sum_toList]
 
 /-!
 ## Prompt
